The Homotopy Extension Property
===============================

In this final section of the chapter we will actually prove a few things, including 
the two criteria for homotopy equivalence described above. The proofs depend upon 
a technical property that arises in many other contexts as well. Consider the following 
problem. Suppose one is given a map :math:`f_0:X \rightarrow Y`, and on a subspace :math:`A \subset X` one is also 
given a homotopy :math:`f_t:A \rightarrow Y` of :math:`f_0 \mid A` that one would like to extend to a homotopy 
:math:`f_t:X \rightarrow Y` of the given :math:`f_0`. If the pair :math:`(X,A)` has the **homotopy extension property**. Thus 
:math:`(X,A)` has the homotopy extension property if every pair of maps :math:`X \times \{0\} \rightarrow Y` and 
:math:`A \times I \rightarrow Y` that agree on :math:`A \times \{0\}` can be extended to a map :math:`X \times I \rightarrow Y`.

    *A pair* :math:`(X,A)` *has the homotopy extension property if and only if* :math:`X \times \{0\} \cup A \times I` *is a
    retract of* :math:`X \times I`.

For one 